Increase number of available inodes
We only had 320 inodes, which is easy to fill up.

src/fs/super.dfy
@@ -52,9 +52,14 @@ module FsKinds {
   }
 
   // we initialize the superblock this way to get named arguments
-  const super := Super.zero.(inode_blocks:=10, data_bitmaps:=6)
+  const super := Super.zero.(inode_blocks:=30, data_bitmaps:=6)
   lemma super_valid()
     ensures super.Valid()
+  {}
+  lemma super_size()
+    ensures super.num_inodes == 960;
+    ensures super.num_data_blocks
+        * 4096 / (1000*1000) == 805 /* MB */
   {}
 
   datatype SuperBlock = SuperBlock(info: Super, actual_blocks: uint64)
@@ -110,8 +115,8 @@ module FsKinds {
   // computes a big int every time it's referenced, which shows up in the CPU
   // profile...
   const super_num_data_blocks: uint64 := 6*(4096*8)
-  const super_data_bitmap_start: uint64 := 513 + 1 + 10;
-  const super_data_start: uint64 := 513 + 1 + 10 + 6;
+  const super_data_bitmap_start: uint64 := 513 + 1 + 30;
+  const super_data_start: uint64 := 513 + 1 + 30 + 6;
   lemma super_consts_ok()
     ensures super_num_data_blocks as nat == super.num_data_blocks
     ensures super_data_bitmap_start as nat == super.data_bitmap_start
